more api update

fstar/api/MLS.API.fsti
@@ -1,21 +1,48 @@
 module MLS.API
 
-type uint64
-type bytes
-type entropy
+/// Basic types that will be completed later
+val uint64: eqtype
+val bytes: eqtype
 val result: Type -> Type
 
+/// Entropy typeclass
+
+class entropy (t:Type) = {
+  extract_entropy: t -> nat -> (bytes & t)
+}
+
+/// Types that are abstract
 type mls_group
-type pending_proposal
-type framing_params
-type commit_params
+type unvalidated_proposal
+type validated_proposal
 type unvalidated_commit
 type validated_commit
+type credential
+type credential_pair
+type signature_keypair
+
+type framing_params = {
+  // Should we encrypt the message?
+  encrypt: bool;
+  // How much padding to add
+  padding_size: nat;
+}
+
+type commit_params = {
+  // Extra proposals to include in the commit
+  proposals: unit; //TODO
+  // Should we inline the ratchet tree in the Welcome messages?
+  inline_tree: bool;
+  // Should we force the UpdatePath even if we could do an add-only commit?
+  force_update: bool;
+  // Options for the generation of the new leaf node
+  leaf_node_options: unit; //TODO
+}
 
 noeq
 type processed_message_content =
   | ApplicationMessage: bytes -> processed_message_content
-  | Proposal: pending_proposal -> processed_message_content
+  | Proposal: unvalidated_proposal -> processed_message_content
   | Commit: unvalidated_commit -> processed_message_content
 
 noeq
@@ -25,25 +52,66 @@ type processed_message = {
   sender: unit; //TODO
   authenticated_data: bytes;
   content: processed_message_content;
-  credential: unit; //TODO
+  credential: credential;
 }
+
+(*** Credentials ***)
+
+val generate_signature_keypair:
+  #entropy_t:Type0 -> {|entropy entropy_t|} ->
+  entropy_t ->
+  entropy_t & result signature_keypair
+
+val get_signature_public_key:
+  signature_keypair ->
+  bytes
+
+val mk_basic_credential:
+  signature_keypair -> identity:bytes ->
+  result credential_pair
+
+val mk_x509_credential:
+  signature_keypair -> x509_chain:list bytes ->
+  result credential_pair
+
+val get_public_credential:
+  credential_pair ->
+  credential
+
+// TODO inspect a credential
 
 (*** Group creation ***)
 
-// TODO: identity stuff? signature key?
 val create_group:
-  entropy ->
-  result mls_group
+  #entropy_t:Type0 -> {|entropy entropy_t|} ->
+  entropy_t ->
+  credential_pair ->
+  entropy_t & (result mls_group)
 
-let key_callback = bytes -> option bytes
+let key_lookup = bytes -> option bytes
 val join_group:
-  bytes ->
-  key_callback ->
+  welcome:bytes ->
+  key_lookup ->
   result mls_group
 
 val join_with_external_commit:
   unit -> //TODO
   result mls_group
+
+(*** Create key package ***)
+
+type create_key_package_result = {
+  key_package: bytes;
+  // key and value to be added to the store
+  keystore_key: bytes;
+  keystore_value: bytes;
+}
+
+val create_key_package:
+  #entropy_t:Type0 -> {|entropy entropy_t|} ->
+  entropy_t ->
+  credential_pair ->
+  entropy_t & (result create_key_package_result)
 
 (*** Export data from the group ***)
 
@@ -56,6 +124,10 @@ val epoch_authenticator:
   mls_group ->
   result bytes
 
+val epoch:
+  mls_group ->
+  result uint64
+
 // TODO: get resumption PSK? Or is it useless for the application?
 
 // TODO: not sure how it is useful. Maybe for external commits?
@@ -65,7 +137,25 @@ val group_info:
 
 (*** Inspect commit ***)
 
-// TODO, take inspiration from OpenMLS or mls-rs?
+val get_new_credentials:
+  unvalidated_commit ->
+  result (list credential)
+
+// TODO:
+// - roster update (added, updated, removed members)
+// - added psk
+// - is pending reinit
+// - is active (am I still present in the group)
+// - new epoch
+// - unused proposals
+
+(*** Inspect proposal ***)
+
+// TODO more getters
+
+val get_new_credential:
+  unvalidated_proposal ->
+  result (option credential)
 
 (*** Process messages ***)
 
@@ -79,57 +169,72 @@ val i_hereby_declare_that_i_have_checked_the_new_credentials_and_validate_the_co
   unvalidated_commit ->
   validated_commit
 
-val queue_new_proposal:
-  mls_group ->
-  pending_proposal ->
-  result mls_group
-
 val merge_commit:
   mls_group ->
   validated_commit ->
   result mls_group
 
+val i_hereby_declare_that_i_have_checked_the_new_credentials_and_validate_the_proposal:
+  unvalidated_proposal ->
+  validated_proposal
+
+val queue_new_proposal:
+  mls_group ->
+  validated_proposal ->
+  result mls_group
+
 (*** Send messages ***)
 
-// TODO: encryption options, such as padding?
+// Authenticated data is sent in plaintext!
 val send_application_message:
+  #entropy_t:Type0 -> {|entropy entropy_t|} ->
+  entropy_t ->
   mls_group ->
   framing_params ->
   message:bytes ->
   authenticated_data:bytes ->
-  bytes
+  entropy_t & bytes
 
 (*** Send proposals ***)
 
 val propose_add_member:
+  #entropy_t:Type0 -> {|entropy entropy_t|} ->
+  entropy_t ->
   mls_group ->
   framing_params ->
   key_package:bytes ->
-  result bytes
+  entropy_t & (result bytes)
 
 val propose_remove_member:
+  #entropy_t:Type0 -> {|entropy entropy_t|} ->
+  entropy_t ->
   mls_group ->
   framing_params ->
-  removed:unit -> // TODO
-  result bytes
+  removed:credential ->
+  entropy_t & (result bytes)
 
 val propose_remove_myself:
+  #entropy_t:Type0 -> {|entropy entropy_t|} ->
+  entropy_t ->
   mls_group ->
   framing_params ->
-  result bytes
+  entropy_t & (result bytes)
 
 val propose_external_psk:
+  #entropy_t:Type0 -> {|entropy entropy_t|} ->
+  entropy_t ->
   mls_group ->
   framing_params ->
   psk:unit -> // TODO
-  result bytes
+  entropy_t & (result bytes)
 
 (*** Create commit ***)
 
 val create_commit:
+  #entropy_t:Type0 -> {|entropy entropy_t|} ->
+  entropy_t ->
   mls_group ->
   framing_params ->
   commit_params ->
-  validated_commit // TODO, if validated we need to validate proposals somehow?
-
+  entropy_t & bytes
 
